src/Soundness.v
@@ -93,7 +93,7 @@ Definition expr_list_soundness n el ρ σ ψ r Γ Σ U Tl :=
         (Tl, Σ') ⊨ vl.
 
 Definition init_soundness n C flds I ρ σ Γ Σ r :=
-  forall Args Flds Mtds ω,
+  forall Args Flds Mtds ω DoneFlds,
     (Γ, Σ) ⊨ ρ ->
     Σ ⊨ σ ->
 
@@ -103,14 +103,18 @@ Definition init_soundness n C flds I ρ σ Γ Σ r :=
     ct C = class Args Flds Mtds ->
     getObj σ I = Some (C, ω) ->
     dom ω + dom flds = dom Flds ->
-    (Σ ⊨ I : cool (dom ω)) ->
+    DoneFlds ++ flds = Flds ->
+    getType Σ I = Some (C, cool (dom ω)) ->
 
     init C flds I ρ σ n = r ->
     r <> Timeout_i ->
 
-    exists Σ' σ',
+    exists Σ' σ' ω',
       r = Success_i σ' /\
-        Σ ≼ Σ' /\ Σ ≪ Σ' /\ Σ ▷ Σ' /\ (Σ' ⊨ σ') /\ wf σ' /\
+        Σ ≼ Σ' /\ Σ ≪ Σ' /\ ([I↦(C,cool (dom Flds))]Σ ▷ Σ') /\ (Σ' ⊨ σ') /\ wf σ' /\
+        getObj σ' I = Some (C, ω') /\
+        dom ω' = dom Flds /\
+        getType Σ' I = Some (C, cool (dom Flds)) /\
         ( forall L σ0,
             (* Hypothesis *)
             ((σ0, L) ⋖ (σ, (codom ρ) ∪ {I})) ->
@@ -118,8 +122,7 @@ Definition init_soundness n C flds I ρ σ Γ Σ r :=
             dom σ0 <= dom σ ->
             (* Conclusions *)
             ((σ0, L) ⋖ (σ', (codom ρ) ∪ {I})) /\
-              (σ0 ⇝ σ' ⋖ L) /\
-              (exists ω', getObj σ' I = Some (C, ω') /\ dom ω' = dom Flds)).
+              (σ0 ⇝ σ' ⋖ L)).
 
 
 Theorem soundness:
@@ -163,7 +166,7 @@ Proof with (
     (* Destruct evaluation of e *)
     destruct_eval H__eval v' σ';
       lets (Σ0 & v0 & σ0 & H__r & H__mn0 & H__stk0 & H__aty0 & H__st0 & H__wf0 & H__v0) :
-      IH__expr HT__e H0 H1 H3 H__eval; try inverts H__r ...
+      IH__expr HT__e H0 H1 H3 H__eval; try inverts H__r; try congruence ...
     eapply eval_implies_evalp in H__eval.
     lets (?C & ?ω & ?μ & H__obj & ? & H__ot): (proj2 H__st0) v0 ...
     rewrite H__obj in H6 |- *.
@@ -185,7 +188,7 @@ Proof with (
         inverts H__ot.
       * (* cool Ω *)
         destruct (getVal ω f) as [v1 |] eqn:H__getVal; [|apply nth_error_None in H__getVal] ...
-        lets: H14 H__getVal H__fieldType...
+        lets: H16 H__getVal H__fieldType...
         exists Σ0, v1, σ0; splits ...
       * (* hot *)
         lets [v1 [ ]]: H16 H__fieldType... rewrite_any.
@@ -195,7 +198,7 @@ Proof with (
         exists Σ0, v1, σ0; splits ...
       * (* cool Ω1 + Ω2 *)
         destruct (getVal ω f) as [v1 |] eqn:H__getVal; [|apply nth_error_None in H__getVal] ...
-        lets: H14 H__getVal H__fieldType...
+        lets: H16 H__getVal H__fieldType...
         exists Σ0, v1, σ0; splits ...
 
   - (* e = mtd e m l *)
@@ -208,7 +211,7 @@ Proof with (
     (* Destruct evaluation of e0 *)
     destruct_eval H__eval0 v σ';
       lets (Σ0 & v0 & σ0 & H__r & H__mn0 & H__stk0 & H__aty0 & H__st0 & H__wf0 & H__v0) :
-      IH__expr HT__e0 H0 H1 H3 H__eval0; try inverts H__r ...
+      IH__expr HT__e0 H0 H1 H3 H__eval0; try inverts H__r; try congruence ...
     eapply eval_implies_evalp in H__eval0.
     lets H__pM0: pM_theorem H__eval0.
     lets (?C & ?ω & ?μ & H__obj & ? & ?): (proj2 H__st0) v0 ...
@@ -225,7 +228,7 @@ Proof with (
     lets (?T & ?T & ? & ? & ?): H__mn0 ψ ...
     destruct_eval H__eval1 vl σ';
       lets (Σ1 & args_val & σ1 & H__r & H__mn1 & H__stk1 & H__aty1 & H__st1 & H__wf1 & H__v1) :
-      IH__list HT__args H__env0 H__st0 H__wf0 H__eval1; try inverts H__r ...
+      IH__list HT__args H__env0 H__st0 H__wf0 H__eval1; try inverts H__r; try congruence ...
     eapply eval_list_implies_evalp in H__eval1. eval_dom; eval_wf.
 
     (* Extract typing for method body from Ξ (well-typed) *)
@@ -238,10 +241,10 @@ Proof with (
     lets (?T & ?T & ? & ? & ?): H__mn1 ψ...
     lets (?T & ?T & ? & ? & ?): H__mn1 v0...
     assert (HT__em': (Args, (C1, μ__m)) ⊢ e__m : (C, μ__r)) by (eapply weakening with (Γ := Flds); eauto with typ).
-    assert (codom args_val ∪ {v0} ⪽ σ1) by (apply storeSubset_union; [eapply wf_theorem_list |]; eauto with wf).
+    assert (codom args_val ∪ {v0} ⪽ σ1). { ss... eapply wf_theorem_list... }
     destruct (⟦ e__m ⟧ (σ1, args_val, v0 )( n)) as [ | | σ' v' ] eqn:H__eval2; try congruence;
     lets (Σ2 & v2 & σ2 & H__r & H__mn2 & H__stk2 & H__aty2 & H__st2 & H__wf2 & H__v2) :
-      IH__expr HT__em' H__v1 H__st1 H__wf1 H__eval2; try inverts H__r ...
+      IH__expr HT__em' H__v1 H__st1 H__wf1 H__eval2; try inverts H__r; try congruence ...
     eapply eval_implies_evalp in H__eval2. clear H6.
 
     (* Result *)
@@ -263,30 +266,111 @@ Proof with (
 
     (* Induction on the typing judgment *)
     eapply t_new_inv in H as
-        (Args & Flds & Mts & argsTs & ?μ & ? & H__ct & HT__args & HS__args & H__mode) ...
+        (Args & Flds & Mtds & argsTs & ?μ & ? & H__ct & HT__args & HS__args & H__mode) ...
 
     (* Destruct evaluation of arguments *)
     destruct_eval H__eval1 vl σ';
-      lets (Σ1 & args_val & σ1 & H__r & H__mn1 & H__stk1 & H__aty1 & H__st1 & H__wf1 & H__v1) :
-      IH__list HT__args H0 H1 H3 H__eval1; try inverts H__r ...
+      lets (Σ1 & args_val & σ1 & H__r & H__mn1 & H__stk1 & H__aty1 & H__st1 & H__wf1 & H__argsval) :
+      IH__list HT__args H0 H1 H3 H__eval1; try inverts H__r; try congruence ...
     inverts H... rename c into C.
     rewrite H__ct in H6 |- *.
     eapply eval_list_implies_evalp in H__eval1...
 
     (* Destruct result of initialization *)
-    assert ((codom args_val ∪ {dom σ1}) ⪽ σ1 ++ [(C, [])]). {
-      lets [ ]: wf_theorem_list H__eval1...
-      eapply storeSubset_union; [eapply storeSubset_trans with σ1 |]; update_dom...
-      eapply storeSubset_singleton3; rewrite dom_app... }
-    remember (Σ1 ++ [(C, cool 0)]) as Σ1'.
-    assert (Σ1' ⊨ σ1 ++ [(C, [])]).
-    lets: getObj_last σ1 C ([]:Env).
-    destruct (init C Flds dom σ1 args_val (σ1 ++ [(C, [])]) n) as [ | | σ2] eqn:Heq;
-      rewrite Heq in H6 |- *; [congruence | |].
-    + lets: IH__init H__v1 Heq...
+    remember (Σ1 ++ [(C, cool 0)]) as Σ2.
+    remember (σ1 ++ [(C, [])]) as σ2...
+    assert ((codom args_val ∪ {dom σ1}) ⪽ σ2). {
+      subst; ss; updates... apply ss_trans with σ1; updates...
+      eapply wf_theorem_list... }
+    assert (H__mn2:  Σ1 ≼ Σ2). {
+        subst. intros l0 H__l0.
+        lets [T ?]: getType_Some H__l0. exists T, T; splits...
+        rewrite getType_last2... }
+    lets H__env2: env_typing_monotonicity H__mn2 H__argsval.
+    assert (H__st2: Σ2 ⊨ σ2). { (* could be a lemma *)
+      subst. split; updates...
+      intros l H__l.
+      destruct_eq (l = dom σ1); subst; updates.
+      - rewrite (proj1 H__st1) getType_last.
+        exists C ([]:Env) (cool 0); splits...
+        apply ot_cool; simpl => //.
+        intros [ ] ? ? ? Hf; inverts Hf.
+      - rewrite getObj_last2...
+        rewrite getType_last2...
+        lets (?C & ?ω & ?μ & ? & ? & ?): (proj2 H__st1) l...
+        repeat eexists... }
+    lets H__wf2: wf_add_empty C H__wf1. rewrite -Heqσ2 in H__wf2.
+    lets: getObj_last σ1 C ([]: Env).
+    destruct (init C Flds dom σ1 args_val (σ1 ++ [(C, [])]) n) as [ | | σ3] eqn:Heq;
+      rewrite Heq in H6 |- *; try congruence;
+    specialize (IH__init C Flds (dom σ1) args_val σ2 argsTs Σ2);
+      lets (Σ4 & σ4 & ω4 & H__r & H__mn4 & H__stk4 & H__aty4 & H__st4 & H__wf4 & H__obj4 & H__dom4 & H__getType4 & H__scp4):
+      IH__init ([]: list Field) H__env2 H__st2 H__ct; subst; simpl...
+    all: try solve [intros; discriminate].
+    all: try solve [rewrite (proj1 H__st1) getType_last; simpl; reflexivity].
+    inverts H__r.
+
+    (* Promotion *)
+    remember ([dom σ1 ↦ (C, warm)] (Σ4)) as Σ5.
+    assert (H__stk5: Σ4 ≪ Σ5). {
+      subst.
+      intros l H__l. updates... }
+    assert (H__mn5: Σ4 ≼ Σ5). {
+      intros l H__l. subst.
+      lets (? & ?): getType_Some Σ4 l... exists (C1, μ).
+      destruct_eq (dom σ1 = l); subst; updates...
+      exists (C, warm)... }
+    assert (H__aty4': Σ1 ▷ Σ4). {
+      intros l ? ? H__getType.
+      lets: getType_dom H__getType.
+      assert (l <> dom Σ1) by lia.
+      apply H__aty4...
+      rewrite getType_update_diff...
+      rewrite getType_last2... }
+    pose proof (promotion Σ1 Σ4 C (dom σ1) σ4 Args Flds Mtds) as H__promotion...
+    lets (H__aty5 & H__mn5' & H__st5): H__promotion H__ct Σ5... clear H__promotion.
+
+    (* aCyse analysis : warm or hot *)
+    destruct H__mode as [H__warm | H__hots].
+    + (* warm *)
+      exists Σ5, (dom σ1), σ4; splits...
+      * eapply stk_st_trans with Σ1...
+        intros l H__l; subst; updates.
+        destruct_eq (dom σ1 = l); subst; updates.
+        -- left; exists C, (C, warm); updates...
+        -- lets [ ]: H__stk4 H__l; updates...
+           inverts H10. inverts H11. left; exists x, T1; updates...
+      * exists (C, warm); subst; updates...
+
+    + (* hot *)
+      eapply init_implies_initP in Heq. eval_dom. updates...
+      destruct (local_reasoning2 Σ1 Σ5 σ1 σ4 (codom args_val) {dom σ1} ) as
+        (Σ6 & ? & ? & ? & ? & H__vnew)...
+      * eapply wf_theorem_list...
+      * lets H__scp5: scp_theorem_init Heq.
+        lets [? _]: H__scp4 (codom args_val) σ1.
+
+        eapply scp_union_intror, H12... eapply ss_trans with (σ1++[(C,[])]); updates...
 
 
-    admit.
+
+      admit. admit. admit.
+      * exists Σ6, (dom σ1), σ4; splits...
+        -- apply stk_st_trans with Σ1...
+           apply stk_st_trans with Σ5... subst.
+           intros l H__l...
+           lets [|] : H__stk4 l...
+           ++ left. lets (?T & ?T & ? & ? & ?): H__mn5 l...
+              exists C2, (C2, μ)...
+              inverts H14... inverts H17...
+           ++ updates.
+              assert (l = dom σ1 \/ l < dom σ1) as [|] by lia...
+              subst. left.
+              exists C, (C, warm); updates...
+        -- exists (C, hot)...
+           lets: H__vnew (dom σ1) In_singleton... inverts H14. inverts H15. meta.
+           assert (x = C); subst...
+           lets (? & ? & ? & ? & ? & ?): (proj2 H13) (dom σ1)...
 
   - (* e = e1.f = e2; e3 *)
     rename v into f.
@@ -300,7 +384,7 @@ Proof with (
     (* Destruct evaluation of e1 *)
     destruct_eval H__eval1 v' σ';
       lets (Σ1 & v1 & σ1 & H__r & H__mn1 & H__stk1 & H__aty1 & H__st1 & H__wf1 & H__v1) :
-      IH__expr HT__e1 H0 H1 H3 H__eval1; try inverts H__r ...
+      IH__expr HT__e1 H0 H1 H3 H__eval1; try inverts H__r; try congruence ...
     eapply eval_implies_evalp in H__eval1.
     lets (?C & ?ω & ?μ & H__obj & ? & H__ot): (proj2 H__st1) v1 ...
 
@@ -310,7 +394,7 @@ Proof with (
     eval_dom. eval_wf...
     destruct_eval H__eval2 v' σ';
       lets (Σ2 & v2 & σ2 & H__r & H__mn2 & H__stk2 & H__aty2 & H__st2 & H__wf2 & H__v2) :
-      IH__expr HT__e2 H__env1 H__st1 H__wf1 H__eval2; try inverts H__r ...
+      IH__expr HT__e2 H__env1 H__st1 H__wf1 H__eval2; try inverts H__r; try congruence ...
     eapply eval_implies_evalp in H__eval2. eval_dom; eval_wf.
     lets (?T & ?T & ? & ? & ?): H__mn2 ψ ...
 
@@ -319,7 +403,7 @@ Proof with (
     destruct (getObj σ2 v1) as [[?C ?ω] |] eqn:H__getObj.
 
     + (* Useful assignment *)
-      remember ([v1 ↦ (C1, [f ↦ v2] (ω0))] (σ2)) as σ2'.
+      remember ([v1 ↦ (C1, [f ↦ v2] (ω0))] (σ2)) as σ2'. rewrite -Heqσ2' in H6.
       assert (H__st2': Σ2 ⊨ σ2'). {
         subst. rename v1 into l, v2 into v.
         lets [?ω [H__obj2 _]]: pM_theorem H__eval2 H__obj.
@@ -336,17 +420,18 @@ Proof with (
         eapply storeTyping_assgn with (μ0 := μ5) ...
       }
       assert (H__wf2': wf σ2') by (subst; eapply wf_assign; eauto).
-      assert (H__codom' : (codom ρ ∪ {ψ}) ⪽ σ2') by (eapply storeSubset_trans; subst; update_dom; eauto).
+      assert (H__codom' : (codom ρ ∪ {ψ}) ⪽ σ2'). by (subst; ss).
       destruct (⟦ e3 ⟧ (σ2', ρ, ψ )( n)) as [ | | σ' v' ] eqn:H__eval3; try congruence;
         lets (Σ3 & v3 & σ3 & H__r & H__mn3 & H__stk3 & H__aty3 & H__st3 & H__wf3 & H__v3) :
-        IH__expr HT__e3 H__st2' H__eval3; try inverts H__r ...
+        IH__expr HT__e3 H__st2' H__eval3; try inverts H__r; try congruence ...
       (* eapply eval_implies_evalp in H__eval3. eval_dom; eval_wf.*)
+      subst.
       exists Σ3, v3, σ3; subst; splits...
 
     + (* Useless assignment *)
       destruct (⟦ e3 ⟧ (σ2, ρ, ψ )( n)) as [ | | σ' v' ] eqn:H__eval3; try congruence;
         lets (Σ3 & v3 & σ3 & H__r & H__mn3 & H__stk3 & H__aty3 & H__st3 & H__wf3 & H__v3) :
-        IH__expr HT__e3 H__st2 H__wf2 H__eval3; try inverts H__r ...
+        IH__expr HT__e3 H__st2 H__wf2 H__eval3; try inverts H__r; try congruence ...
       eapply eval_implies_evalp in H__eval3. eval_dom; eval_wf.
       exists Σ3, v3, σ3; splits...
 
@@ -361,7 +446,7 @@ Proof with (
     (* Destruct evaluation of head *)
     destruct_eval H__eval v' σ';
       lets (Σ0 & v & σ0 & H__r & H__mn0 & H__stk0 & H__aty0 & H__st0 & H__wf0 & H__v0) :
-      IH__expr H14 H0 H1 H3 H__eval; try inverts H__r ...
+      IH__expr H14 H0 H1 H3 H__eval; try inverts H__r; try congruence ...
     eapply eval_implies_evalp in H__eval. eval_dom.
 
     (* Destruct evaluation of tail *)
@@ -369,7 +454,7 @@ Proof with (
     lets H__env0: env_typing_monotonicity H__mn0 H0.
     destruct (⟦_ el _⟧ (σ0, ρ, ψ )( n)) as [ | | σ' vl' ] eqn:H__eval1; try congruence;
     lets (Σ1 & vl & σ1 & H__r & H__mn1 & H__stk1 & H__aty1 & H__st1 & H__wf1 & H__v1):
-      IH__list H12 H__env0 H__st0 H__wf0 H__eval1; try inverts H__r ...
+      IH__list H12 H__env0 H__st0 H__wf0 H__eval1; try inverts H__r; try congruence ...
 
     (* Result *)
     exists Σ1, (v::vl), σ1; splits...
@@ -377,16 +462,97 @@ Proof with (
     apply et_cons...
 
   - (* init [] *)
-    exists Σ σ; splits...
-    intros; splits...
+    updates. simpl in *. repeat rewrite Nat.add_0_r in H5 |- *.
+    exists Σ, σ, ω. splits...
+    + intros l ?C Ω H__getType.
+      destruct_eq (I = l); subst; updates...
+      rewrite getType_update_same in H__getType... steps.
+    + splits... congruence.
 
-  - (* init f::flds *)
+  - (* init_cons *)
+    destruct f as [μ__f e].
 
+    (* Extract typing from the well-typed classes *)
+    pose proof (typable_classes C) as HT__C. rewrite H3 in HT__C.
+    destruct HT__C as [HT__Field _].
+    eapply T_Fields_In in HT__Field. unfold T_Field in HT__Field.
+    eapply weakening with (Γ' := Γ) in HT__Field; [| intros [ ] Tx Hf; inverts Hf].
+    rename HT__Field into HT__e.
+    updates.
+    assert (H__doms: dom DoneFlds = dom ω). {
+      eapply plus_reg_l.
+      rewrite Nat.add_comm.
+      rewrite <- H5... } rewrite H__doms in HT__e |- *.
 
+  (* Destruct evaluation of e *)
+    destruct_eval H__eval v' σ';
+      lets (Σ0 & v0 & σ0 & H__r & H__mn0 & H__stk0 & H__aty0 & H__st0 & H__wf0 & H__v0) :
+       IH__expr HT__e H0 H1 H2 H__eval; try inverts H__r; try congruence ...
+    eapply eval_implies_evalp in H__eval.
+    lets H__eM: eM_theorem H__eval. lets [ω' [ ]]: H__eM H4.
+    lets: monotonicity_dom H__mn0.
+    lets (? & ? & ? & ? & ?): H__mn0 I...
+    lets (?C & ?ω & ?μ & ? & ? & ?): (proj2 H__st0) I...
+    eval_dom; eval_wf.
 
+    (* Use field initialization lemma *)
+    unfold assign_new in *.
+    rewrite H7 in H9 |- *.
+    lets H__env0: env_typing_monotonicity H__mn0 H.
+    clear IH__expr IH__list.
+    lets: H__aty0 I H15.
+    assert (H__field: fieldType C (dom ω) = Some (C0, μ)). {
+      unfold fieldType. rewrite H3.
+      rewrite nth_error_app2... rewrite H__doms -minus_diag_reverse.
+      simpl => //.
+    }
+    rewrite H12 in H10, H__field.
+    remember ([I ↦ (C, cool (S dom ω'))] (Σ0)) as Σ1.
+    remember ([I ↦ (C, ω' ++ [v0])] (σ0)) as σ1.
+    lets (H__st1 & H__mn1 & H__stk1): field_initialization v0 H__st0 H10 H__field Σ1;
+      unfold assign_new; auto; [|steps|]...
 
-
-
-
-
-Admitted.
+    (* Use induction hypothesis *)
+    lets: env_typing_monotonicity H__mn1 H__env0.
+    assert ( wf [I ↦ (C, ω' ++ [v0])] (σ0)). {
+      eapply wf_assign_new with (flds := flds)... updates... }
+    specialize (IH__init
+                  C flds I ρ
+                  σ1
+                  Γ Σ1
+                  (init C flds I ρ σ1 n)
+                  Args (DoneFlds++(field (C0,μ) e)::flds) Mtds
+                  (ω'++[v0])
+                  (DoneFlds ++ [field (C0, μ) e])).
+    subst; modus.
+    destruct IH__init
+      as (Σ2 & σ2 & ω2 & H__r & H__mn2 & H__stk2 & H__aty2 & H__st2 & H__wf2 & H__obj2 & H__dom2 & H__getType2 & H__scp2)...
+    + rewrite getObj_update_same...
+    + updates...
+    + rewrite app_assoc_reverse. simpl => //.
+    + rewrite getType_update_same; updates...
+      rewrite Nat.add_1_r...
+    + (* Result *)
+      updates.
+      rewrite H__doms in H__aty2, H__getType2.
+      lets H__initP: H__r.
+      eapply init_implies_initP in H__initP.
+      lets H__scpInit: scp_theorem_init H__initP.
+      lets [ ]: scp_theorem H__eval...
+      exists Σ2, σ2, ω2; splits...
+      * intros l ?C Ω H__getType.
+        destruct_eq (I = l); subst; updates.
+        -- rewrite getType_update_same in H__getType... steps.
+        -- eapply H__aty0 in H__getType.
+           eapply H__aty2. updates...
+      * splits...
+        intros.
+        eapply H__scp2...
+        -- eapply scp_add_env; eauto with lia wf; updates.
+           ++ apply H23.
+           ++ eapply scp_trans; eauto with scp.
+           ++ eapply scp_trans; eauto with scp.
+        -- eapply scp_pr_trans; eauto.
+           eapply scp_pr_trans; eauto.
+           unfold scoping_preservation; intros; eauto with scp.
+Qed.
